VProg/Instructions.v
@@ -8,85 +8,72 @@ Import SL.Tactics.
 Section Read.
   Context [CT : CP.context] (p : ptr).
 
-  Inductive Read_Spec (ctx : CTX.t) : i_spec_t memdata ctx -> Prop
+  Inductive Read_Spec (ctx : CTX.t) (F : i_spec_t memdata ctx) : Prop
     := Read_SpecI
     (d : memdata)
-    (img : Sub.t ctx)
-    (ij : CTX.Inj.ieq [CTX.mka (SLprop.cell p, d)] ctx img):
-    Read_Spec ctx {|
-      sf_csm  := Sub.const ctx false;
+    (IJ : InjPre_Frame_Spec [CTX.mka (SLprop.cell p, d)] ctx {|
+      sf_csm  := Vector.cons _ false _ (Vector.nil _) <: Sub.t [_];
       sf_prd  := fun _ => nil;
       sf_spec := FP.Ret (TF.mk _ d Tuple.tt);
-    |}.
+    |} F).
 
   Program Definition Read : instr CT memdata := {|
     i_impl := CP.Read p;
     i_spec := fun ctx => Read_Spec ctx;
   |}.
   Next Obligation.
-    destruct SP; do 2 intro; simpl in *.
-    eapply SP.CFrame with (fr := CTX.sl (CTX.sub ctx (Sub.neg img))).
-    - eapply SP.Read with (d := d).
-    - eassert (IEq : SLprop.eq _ _). {
-        etransitivity. apply (CTX.Inj.ieqE ij).
-        simpl; SL.normalize.
-      }
-      split; simpl.
-      + rewrite CTX.sl_split with (s := img).
-        apply SLprop.star_morph_imp. 2:reflexivity.
-        rewrite IEq; reflexivity.
-      + intro. SL.normalize. Intro ->.
-        unfold sf_post; simpl; SL.normalize.
-        Apply. assumption.
-        etransitivity. apply SLprop.star_morph_imp. 2:reflexivity. 
-        eapply SLprop.imp_morph. symmetry in IEq; exact IEq. 1,2:reflexivity.
-        rewrite <- CTX.sl_split.
-        unfold Sub.neg, Sub.const; rewrite Vector.map_const; simpl.
-        rewrite Sub.sub_const_true.
-        reflexivity.
+    destruct SP.
+    apply (Tr_InjPre_Frame IJ); clear IJ.
+    do 2 intro; cbn in *.
+    eapply SP.Cons.
+      { apply SP.Read with (d := d). }
+    split; cbn.
+    - SL.normalize; reflexivity.
+    - intro; SL.normalize.
+      Intro ->.
+      Apply PRE.
+      reflexivity.
   Qed.
 End Read.
 
 Local Ltac build_Read :=
-  simple refine (@Read_SpecI _ _ _ _ _);
-  [ shelve | shelve | (* ij *) CTX.Inj.build ].
+  simple refine (Read_SpecI _ _ _ _ _);
+  [ shelve | (*IJ *) Tac.build_InjPre_Frame; Tac.cbn_refl ].
 
 Section Write.
   Context [CT : CP.context] (p : ptr) (d : memdata).
 
-  Inductive Write_Spec (ctx : CTX.t) : i_spec_t unit ctx -> Prop
+  Inductive Write_Spec (ctx : CTX.t) (F : i_spec_t unit ctx) : Prop
     := Write_SpecI
     (d0 : memdata)
-    (csm : Sub.t ctx)
-    (ij : CTX.Inj.ieq [CTX.mka (SLprop.cell p, d0)] ctx csm):
-    Write_Spec ctx {|
-      sf_csm  := csm;
+    (IJ : InjPre_Frame_Spec [CTX.mka (SLprop.cell p, d0)] ctx {|
+      sf_csm  := Vector.cons _ true _ (Vector.nil _) <: Sub.t [_];
       sf_prd  := fun _ => [Vprop.mk (SLprop.cell p)];
       sf_spec := FP.Ret (TF.mk (fun _ => [memdata]) tt (d, tt));
-    |}.
+    |} F).
 
   Program Definition Write : instr CT unit := {|
     i_impl := CP.Write p d;
     i_spec := fun ctx => Write_Spec ctx;
   |}.
   Next Obligation.
-    destruct SP; do 2 intro; simpl in *.
-    eapply SP.CFrame with (fr := CTX.sl (CTX.sub ctx (Sub.neg csm))).
-    - eapply SP.Write with (d0 := d0).
-    - split; unfold sf_post, sf_post_ctx, sf_rsel; simpl.
-      + rewrite CTX.sl_split with (s := csm).
-        apply SLprop.star_morph_imp. 2:reflexivity.
-        rewrite (CTX.Inj.ieqE ij); simpl; SL.normalize; reflexivity.
-      + intros []; SL.normalize.
-        Apply (d, tt).
-        Apply. assumption.
-        reflexivity.
+    destruct SP.
+    apply (Tr_InjPre_Frame IJ); clear IJ.
+    do 2 intro; cbn in *.
+    eapply SP.Cons.
+      { apply SP.Write with (d0 := d0). }
+    split; cbn.
+    - SL.normalize; reflexivity.
+    - intros [].
+      Apply (d, tt).
+      Apply PRE.
+      SL.normalize; reflexivity.
   Qed.
 End Write.
 
 Local Ltac build_Write :=
-  simple refine (@Write_SpecI _ _ _ _ _ _);
-  [ shelve | shelve | (* ij *) CTX.Inj.build ].
+  simple refine (Write_SpecI _ _ _ _ _ _);
+  [ shelve | (* IJ *) Tac.build_InjPre_Frame; Tac.cbn_refl ].
 
 Module Tactics.
   #[export] Hint Extern 1 (Read_Spec    _ _ _) => build_Read   : HasSpecDB.
